




A decorative graphic on the left side of the slide, consisting of a network of white lines and small circles on a dark blue background, resembling a circuit board or a tree structure.

# RECURRENCE RELATIONS

zyBooks Chapter: 8.2, 8.15



# LOGISTICS

- Lab 1 – TONIGHT at 11:59pm (~5 hrs, NO extension)
  - HW 7 – due next Monday, July 6 at 11:59pm
- 
- 
- 

# RECAP

- Recurrence relation
  - A rule that defines a term  $a_n$  as a function of previous terms in the sequence.
  - Linear
  - Homogenous
- Recursive form
- Closed form
- Recursive Form of LHRR  $\rightarrow$  Closed Form

**Q:** Is the following recurrence relation linear and homogenous?

$$s_0 = 3$$

$$s_1 = 10$$

$$s_n = 7 s_{n-1} - 12 s_{n-2} \text{ for } n \geq 2$$

**Q:** Find the closed form

$$s_0 = 3$$

$$s_1 = 10$$

$$s_n = 7s_{n-1} - 12s_{n-2} \text{ for } n \geq 2$$

**Step 0:** Is it a LHRR?

Yes, LHRR, **degree = 2**

**Step 1:** Assume  $s_n = c * x^n$

**Step 2:** Substitute  $s_n = c * x^n$  to find  $x$

$$\text{Hence, } c * x^n = 7 * c * x^{n-1} - 12 * c * x^{n-2}$$

$$x^n = 7x^{n-1} - 12x^{n-2} \quad (\text{divide } c \text{ for both sides})$$

$$x^2 = 7x - 12 \quad (\text{divide } x^{n-2} \text{ for both sides})$$

$$x^2 - 7x + 12 = 0$$

$$(x - 4)(x - 3) = 0$$

Therefore, we have  $x = 4$  and  $x = 3$ .

$$\text{Hence, } s_n = c_1 * 4^n + c_2 * 3^n$$

**Step 3:** Use the base case to find  $c$

$$s_0 = c_1 * 4^0 + c_2 * 3^0 = 3 \rightarrow c_1 + c_2 = 3$$

$$s_1 = c_1 * 4^1 + c_2 * 3^1 = 10 \rightarrow 4c_1 + 3c_2 = 10$$

$$\text{Therefore, } c_1 = 1, c_2 = 2$$

$$\text{That is, } s_n = 4^n + 2 * 3^n$$

# VERIFY – PROOF BY INDUCTION

Given:

$$s_0 = 3$$

$$s_1 = 10$$

$$s_n = 7s_{n-1} - 12s_{n-2} \text{ for } n \geq 2$$

Prove:

$$s_n = 4^n + 2 * 3^n$$

Prove that

$$7s_{n-1} - 12s_{n-2} = 4^n + 2 * 3^n \text{ for } n \geq 2$$

Base Case:

$$\text{Let } n = 0, \text{ LHS} = 3 = 4^0 + 2 * 3^0 = \text{RHS}$$

$$\text{Let } n = 1, \text{ LHS} = 10 = 4^1 + 2 * 3^1 = \text{RHS}$$

Inductive Steps:

Assume  $s_{k-1}$  is true for some integer  $k, k \geq 2$ .

Then we have  $s_{k-1} = 4^{k-1} + 2 * 3^{k-1}$ .

Assume  $s_{k-2}$  is true for some integer  $k, k \geq 2$ .

Then we have  $s_{k-2} = 4^{k-2} + 2 * 3^{k-2}$ .

Prove that  $s_k = 4^k + 2 * 3^k$  is true for some integer  $k, k \geq 2$ .

# VERIFY – PROOF BY INDUCTION

Given:

$$s_0 = 3$$

$$s_1 = 10$$

$$s_n = 7s_{n-1} - 12s_{n-2} \text{ for } n \geq 2$$

Prove:

$$s_n = 4^n + 2 * 3^n$$

Prove that

$$7s_{n-1} - 12s_{n-2} = 4^n + 2 * 3^n \text{ for } n \geq 2$$

Inductive Steps:

... Then we have  $s_{k-1} = 4^{k-1} + 2 * 3^{k-1}$  and  $s_{k-2} = 4^{k-2} + 2 * 3^{k-2}$ .

Prove that  $s_k = 4^k + 2 * 3^k$  is true for some integer  $k$ ,  $k \geq 2$ .

$$\text{LHS} = 7 * (4^{k-1} + 2 * 3^{k-1}) - 12 * (4^{k-2} + 2 * 3^{k-2})$$

$$= 7 * 4^{k-1} + 14 * 3^{k-1} - 12 * 4^{k-2} - 24 * 3^{k-2}$$

$$= 7 * 4^{k-1} + 14 * 3^{k-1} - 12 * \frac{1}{4} * 4^{k-1} - 24 * \frac{1}{3} * 3^{k-1}$$

$$= 7 * 4^{k-1} + 14 * 3^{k-1} - 3 * 4^{k-1} - 8 * 3^{k-1}$$

$$= (7 - 3) * 4^{k-1} + (14 - 8) * 3^{k-1}$$

$$= 4 * 4^{k-1} + 6 * 3^{k-1} = 4 * 4^{k-1} + 2 * 3 * 3^{k-1}$$

$$= 4^k + 2 * 3^k = \text{RHS}$$

# CLOSED FORM $\rightarrow$ RECURSIVE FORM

**Q:** Find the recursive form given the closed form:  $g_m = (3m + 1)(m - 1)$

$$\begin{aligned} g_{m-1} &= (3(m-1) + 1)((m-1) - 1) \\ &= (3m - 2)(m - 2) \end{aligned}$$

$$\begin{aligned} g_m - g_{m-1} &= (3m + 1)(m - 1) - (3m - 2)(m - 2) \\ &= 3m^2 - 2m - 1 - (3m^2 - 8m + 4) \\ &= 3m^2 - 2m - 1 - 3m^2 + 8m - 4 \\ &= 6m - 5 \end{aligned}$$

$$g_m = g_{m-1} + 6m - 5 \quad \text{for } m \geq 1$$

$$g_0 = (3 * 0 + 1)(0 - 1) = -1$$



**Q:** Find the recursive form given the closed form:  $g_m = (m + 2)(2m - 1)$

$$\begin{aligned} g_{m-1} &= ((m-1) + 2)(2(m-1) - 1) \\ &= (m+1)(2m-3) \end{aligned}$$

$$\begin{aligned} g_m - g_{m-1} &= (m+2)(2m-1) - (m+1)(2m-3) \\ &= 2m^2 + 3m - 2 - (2m^2 - m - 3) \\ &= 2m^2 + 3m - 2 - 2m^2 + m + 3 \\ &= 4m + 1 \end{aligned}$$

$$g_m = g_{m-1} + 4m + 1 \text{ for } m \geq 1$$

$$g_0 = (0 + 2)(2 * 0 - 1) = -2$$

**Q:** Find the recursive form given the closed form:  $s_n = 4 * 3^n + 3 * 4^n$

Therefore,  $x_1 = 3, x_2 = 4$

So we have  $(x - 3)(x - 4) = 0$

$$x^2 - 7x + 12 = 0$$

$$x^2 = 7x - 12$$

Then we have  $x^n = 7x^{n-1} - 12x^{n-2}$  (multiply both sides by  $x^{n-2}$ )

$$s_n = 7s_{n-1} - 12s_{n-2} \quad \text{for } n \geq 2$$

$$s_0 = 4 * 3^0 + 3 * 4^0 = 7$$

$$s_1 = 4 * 3^1 + 3 * 4^1 = 24$$

$$s_n = c_1 * x_1^n + c_2 * x_2^n$$

\*\*\* LHRR \*\*\*

**Q:** Find the recursive form given the closed form:  $s_n = 3^n + 3 * 2^n$

Therefore,  $x_1 = 3, x_2 = 2$

So we have  $(x - 3)(x - 2) = 0$

$$x^2 - 5x + 6 = 0$$

$$x^2 = 5x - 6$$

Then we have  $x^n = 5x^{n-1} - 6x^{n-2}$  (multiply both sides by  $x^{n-2}$ )

$$s_n = 5s_{n-1} - 6s_{n-2} \quad \text{for } n \geq 2$$

$$s_0 = 3^0 + 3 * 2^0 = 4$$

$$s_1 = 3^1 + 3 * 2^1 = 9$$

**Q:** Find the recursive form given the closed form:  $s_n = 5 * 2^n + 2 * 4^n$

Therefore,  $x_1 = 2, x_2 = 4$

So we have  $(x - 2)(x - 4) = 0$

$$x^2 - 6x + 8 = 0$$

$$x^2 = 6x - 8$$

Then we have  $x^n = 6x^{n-1} - 8x^{n-2}$  (multiply both sides by  $x^{n-2}$ )

$$s_n = 6 s_{n-1} - 8 s_{n-2} \text{ for } n \geq 2$$

$$s_0 = 5 * 2^0 + 2 * 4^0 = 7$$

$$s_1 = 5 * 2^1 + 2 * 4^1 = 18$$